qa/lean/Ragu/Instances/Point/AddIncomplete.lean
@@ -72,7 +72,7 @@ def formal_instance : Core.Statements.GeneralFormalInstance where
       deserializeInput, exportedOperations,
       Circuits.Point.AddIncomplete.circuit, Circuits.Point.AddIncomplete.elaborated, Circuits.Point.AddIncomplete.main,
       Circuits.Element.Square.circuit, Circuits.Element.Square.elaborated, Circuits.Element.Square.main,
-      Circuits.Element.DivNonzero.generalCircuit, Circuits.Element.DivNonzero.elaborated, Circuits.Element.DivNonzero.main,
+      Circuits.Element.DivNonzero.circuit, Circuits.Element.DivNonzero.elaborated, Circuits.Element.DivNonzero.main,
       Circuits.Core.AllocMul.circuit, Circuits.Core.AllocMul.elaborated, Circuits.Core.AllocMul.main,
       Circuits.Element.Mul.circuit, Circuits.Element.Mul.elaborated, Circuits.Element.Mul.main]
     repeat (constructor; rfl)
@@ -83,7 +83,7 @@ def formal_instance : Core.Statements.GeneralFormalInstance where
       deserializeInput, serializeOutput,
       Circuits.Point.AddIncomplete.circuit, Circuits.Point.AddIncomplete.elaborated, Circuits.Point.AddIncomplete.main,
       Circuits.Element.Square.circuit, Circuits.Element.Square.elaborated, Circuits.Element.Square.main,
-      Circuits.Element.DivNonzero.generalCircuit, Circuits.Element.DivNonzero.elaborated, Circuits.Element.DivNonzero.main,
+      Circuits.Element.DivNonzero.circuit, Circuits.Element.DivNonzero.elaborated, Circuits.Element.DivNonzero.main,
       Circuits.Core.AllocMul.circuit, Circuits.Core.AllocMul.elaborated, Circuits.Core.AllocMul.main,
       Circuits.Element.Mul.circuit, Circuits.Element.Mul.elaborated, Circuits.Element.Mul.main]
     repeat (constructor <;> congr)
